Veir/IR/OpInfo.lean
@@ -1,0 +1,17 @@
+module
+
+namespace Veir
+
+/--
+Define a typeclass hasProperties
+-/
+public class OpInfo (opCodeTy : Type)
+    extends Hashable opCodeTy, Repr opCodeTy, Inhabited opCodeTy where
+  propertiesOf : opCodeTy → Type
+  propertiesHash {opCode : opCodeTy} : Hashable (propertiesOf opCode)
+  propertiesDefault {opCode : opCodeTy} : Inhabited (propertiesOf opCode)
+  propertiesRepr {opCode : opCodeTy} : Repr (propertiesOf opCode)
+  propertiesDecideableEq {opCode : opCodeTy} : DecidableEq (propertiesOf opCode)
+  decideableEq : DecidableEq (opCodeTy)
+
+end Veir
