Veir/Rewriter/WellFormed/Rewriter/Operation.lean
@@ -7,17 +7,17 @@ import Veir.Rewriter.InsertPoint
 
 namespace Veir
 
-variable {dT : Type} [HasProperties dT]
-variable {ctx : IRContext dT}
+variable {opInfo : Type} [OpInfo opInfo]
+variable {ctx : IRContext opInfo}
 
 section insertOp
 
-theorem Rewriter.insertOp?_WellFormed (ctx : IRContext dT) (hctx : ctx.WellFormed)
+theorem Rewriter.insertOp?_WellFormed (ctx : IRContext opInfo) (hctx : ctx.WellFormed)
     (newOp : OperationPtr) (ip : InsertPoint)
     (newOpIn : newOp.InBounds ctx := by grind)
     (insIn : ip.InBounds ctx)
     (hwf : ip.block! ctx = some block)
-    (ctxInBounds : ctx.FieldsInBounds) (newCtx : IRContext dT) :
+    (ctxInBounds : ctx.FieldsInBounds) (newCtx : IRContext opInfo) :
     Rewriter.insertOp? ctx newOp ip newOpIn insIn ctxInBounds = some newCtx →
     newCtx.WellFormed := by
   intros heq
@@ -131,7 +131,7 @@ theorem RegionPtr.blockChain_detachOp
     RegionPtr.BlockChain region (Rewriter.detachOp ctx op hctx hIn hasParent) array := by
   apply RegionPtr.blockChain_unchanged (ctx := ctx) hWf <;> grind
 
-theorem Rewriter.detachOp_WellFormed (ctx : IRContext dT) (wf : ctx.WellFormed)
+theorem Rewriter.detachOp_WellFormed (ctx : IRContext opInfo) (wf : ctx.WellFormed)
     (hctx : ctx.FieldsInBounds) (op : OperationPtr)
     (hIn : op.InBounds ctx)
     (hasParent : (op.get ctx hIn).parent.isSome) :
@@ -228,7 +228,7 @@ theorem RegionPtr.blockChain_detachOpIfAttached
   simp only [Rewriter.detachOpIfAttached]
   grind [RegionPtr.blockChain_detachOp]
 
-theorem Rewriter.detachOpIfAttached_WellFormed (ctx : IRContext dT) (wf : ctx.WellFormed)
+theorem Rewriter.detachOpIfAttached_WellFormed (ctx : IRContext opInfo) (wf : ctx.WellFormed)
     (hctx : ctx.FieldsInBounds) (op : OperationPtr)
     (hIn : op.InBounds ctx) :
     (Rewriter.detachOpIfAttached ctx op hctx hIn).WellFormed := by
@@ -357,7 +357,7 @@ theorem OpResultPtr.firstUse!_detachOperands_eq_none_of_firstUse!_eq_none
   split; grind
   apply OpResultPtr.firstUse!_detachOperands_loop_eq_none_of_firstUse!_eq_none hctx (by grind) resIn h
 
-theorem Rewriter.eraseOp_WellFormed (ctx : IRContext dT) (wf : ctx.WellFormed)
+theorem Rewriter.eraseOp_WellFormed (ctx : IRContext opInfo) (wf : ctx.WellFormed)
     (hctx : ctx.FieldsInBounds) (op : OperationPtr)
     (noRegions : op.getNumRegions! ctx = 0)
     (noUses : op.hasUses! ctx = false)
